

\chapter{Stochastic Processes}

\section{Probability}

Probability generating function

\begin{equation}
G_N(s) = \sum_{n=0}^{\infty} p_{n}s^{n}
\end{equation}

\begin{equation}
\frac{dG(s)}{ds} = G^{\prime}(s) = \sum_{n=1}^{\infty}
np_{n}s^{n-1}
\end{equation}


\begin{equation}
\frac{d^2G(s)}{ds^2} = G^{\prime \prime}(s) =
\sum_{n=2}^{\infty}n(n-1)p_{n}s^{n-2}
\end{equation}

\begin{equation}
G_N(1) = \sum_{n=0}^{\infty} p_{n}
\end{equation}

\begin{equation}
G^{\prime}_N(1) = \sum_{n=1}^{\infty} np_{n}=E(N) = \mu
\end{equation}


The random variable N has a binomial distribution with paramtrics
terms m and p. Its probability function is given by
\begin{equation}
p(n) = p_n  = P(N=n) = {m \choose n}p^nq^{m-n}
\end{equation}

Find its probability generating function.

\begin{equation}
G(s) =  \sum_{n=0}^{m} s^n {m \choose n} p^nq^{m-n}
\end{equation}

\begin{equation}
G(s) =  \sum_{n=0}^{m} {m \choose n} (ps)^n q^{m-n}
\end{equation}


\begin{equation}
G(s) =  (q + ps)^m
\end{equation}


\[
(x + y)^k = [{k \choose 0}x^{k}y^{0}] + [{k \choose
	1}x^{k-1}y^{1}] +  \dots + [{k \choose n}x^{k-n}y^{n}] + \dots [{k
	\choose k-1}x^{1}y^{k-1}] + [ {k \choose k}x^{0}y^{k}]
\]

\[
(x + y)^k = \sum_{n=0}^{k} {k \choose n}x^{k-n}y^{n}
\]

\[
(x + y)^3 = \left[{3 \choose 0}x^{3-0}y^{0}\right] + \left[{3
	\choose 1}x^{3-1}y^{1}\right] +  \left[ {3 \choose
	2}x^{3-2}y^{2}\right] + \left[ {3 \choose 3}x^{3-3}y^{3}\right]
\]

\[
(x + y)^3 = x^{3} + 3x^2y + 3xy^2 + y^{3}
\]


\[
\sum_{n=0}^{k} {k \choose n}p^{k-n}q^{n} = (p + q)^k
\]
This result is not interesting because $p+q=1$

\[
(p + q)^k = 1^{k} = 1
\]
However when using terms $ps$ and $q$ we can say:
\[
\sum_{n=0}^{k} {k \choose n}ps^{k-n}q^{n} = (ps + q)^k
\]


\[
{m \choose n}  = \frac{m!}{n! \times (m-n)!} \]

\section{Poisson}

\[ p(x) = \frac{e^{\alpha}\alpha^{x}}{x!} \qquad x = 0, 1,2 \dots
\]

variance and mean are both equal to $\alpha$.

\section{PGF}

\[
G(s) = \frac{1-\alpha(1-s)}{1+\alpha(1+s)}
\]



