\documentclass[]{report}

\voffset=-1.5cm
\oddsidemargin=0.0cm
\textwidth = 480pt

\usepackage{framed}
\usepackage{subfiles}
\usepackage{graphics}
\usepackage{newlfont}
\usepackage{eurosym}
\usepackage{amsmath,amsthm,amsfonts}
\usepackage{amsmath}
\usepackage{color}
\usepackage{amssymb}
\usepackage{multicol}
\usepackage[dvipsnames]{xcolor}
\usepackage{graphicx}
\begin{document}
\chapter{Conditional Probability}
\section{Conditional Probability}

The conditional probability of an event is the probability that an event A occurs given that another event B has already occurred. This type of probability is calculated by restricting the sample space that we’re working with to only the set B.

The formula for conditional probability can be rewritten using some basic algebra. Instead of the formula:

\[P(A | B) = \frac{P(A \cap B) }{P( B )}  \]


\section{Conditional Probability}
Suppose $B$ is an event in a sample space $S$ with $P(B) > 0$.
The probability that an event $A$ occurs once $B$has occurred or, specifically, the
conditional probability of A given $B$ (written $P(A|B)$), is defined as follows:
\[ P(A|B) = \frac{P(A\cap B)}{P(B)}\]

\begin{itemize}
\item This can be expressed as a multiplication theorem
\[ P(A\cap B) = P(A|B)\times P(B) \]
\item The symbol $|$ is a vertical line and does not imply division.
\item Also $P(A|B)$ is not the same as $P(B|A)$.
\end{itemize}
Remark: The Prosecutor's Fallacy , with reference to the O.J. Simpson trial.


What is the probability of one event given that another event occurs? For example, what is the probability of a mouse finding the end of the maze, given that it finds the room before the end of the maze?

This is represented as:


\[P[A | B]\]
or "the probability of A given B."

\[P(A | B) = \frac{P(A\cap B)}{P(B)}\]

If A and B are independent of one another, such as with coin tosses or child births, then:


\[P[A | B] = P[ A ]\]
Thus, "what is the probability that the next child a family bears will be a boy, given that the last child is a boy."

This can also be stacked where the probability of A with several "givens."


\[P[A | B_1, B_2, B_3 ]\]
or "the probability of A given that B1, B2, and B3 are true?"



\begin{itemize}
\item pairwise disjoint sets
\item The addition principle
\end{itemize}


\section{Conditional Probability}

\[ P(X|Y)  = \frac{P(X \mbox{ and } Y)}{P(Y)} \]

Re-arranging
\[ P(X \mbox{ and } Y) =  P(X|Y)\times P(Y) \]
Therefore we can say
\[ P(F \mbox{ and } A) =  P(F|A)\times P(A) \]\\
\[ P(F \mbox{ and } B) =  P(F|B)\times P(B) \]





\[ P(F \mbox{ and } A) =  P(F|A)\times P(A) \]

\[ P(F \mbox{ and } B) =  P(F|B)\times P(B) \]




\[ P(F \mbox{ and } A) =  P(F|A)\times P(A) = 0.80 \times 0.01\]\\
\[ P(F \mbox{ and } A) = 0.008\]

\[ P(F \mbox{ and } B) =  P(F|B)\times P(B) = 0.20 \times 0.03\]\\
\[ P(F \mbox{ and } B) = 0.006\]

%=================================================================================================$
\textbf{Recall:}
\[ P(F) = P(F \mbox{ and } A) + P(F \mbox{ and } B) \]








\[P[A | B]\]
or "the probability of A given B."

\[P(A | B) = \frac{P(A\cap B)}{P(B)}\]

If A and B are independent of one another, such as with coin tosses or child births, then:


\[P[A | B] = P[ A ]\]
Thus, "what is the probability that the next child a family bears will be a boy, given that the last child is a boy."

This can also be stacked where the probability of A with several "givens."


\[P[A | B_1, B_2, B_3 ]\]
or "the probability of A given that B1, B2, and B3 are true?"



%==================================================================%
\section{Algebaic Results}


\subsection{Multiplication Rule}
The multiplication rule is a result used to determine the probability that two events, $A$ and $B$, both occur.
The multiplication rule follows from the definition of conditional probability.\\ \bigskip

The result is often written as follows, using set notation:
\[ P(A|B)\times P(B) = P(B|A)\times P(A) \qquad \left( = P(A \cap B) \right) \]

Recall that for independent events, that is events which have no influence on one another, the rule simplifies to:
\[P(A \cap B)  = P(A)\times P(B) \]


From the first year intake example, check that
\[ P(E|F)\times P(F) = P(F|E)\times P(E)\]
\begin{itemize}
\item $P(E|F)\times P(F) = 0.58 \times 0.38  = 0.22$
\item $P(F|E)\times P(E) = 0.55 \times 0.40  = 0.22$
\end{itemize}

\subsection{Law of Total Probability}
The law of total probability is a fundamental rule relating marginal probabilities to conditional probabilities. The result is often written as follows, using set notation:
\[ P(A)  = P(A \cap B) + P(A \cap B^c) \]

where $P(A \cap B^c)$ is probability that event $A$ occurs and $B$ does not.\\ \bigskip


Using the multiplication rule, this can be expressed as
\[ P(A) = P(A | B)\times P(B) + P(A | B^{c})\times P(B^{c}) \]


From the first year intake example , check that
\[ P(E)  = P(E \cap M) + P(E \cap F) \]
with $ P(E) = 0.40$, $ P(E \cap M) = 0.18$ and  $ P(E \cap F) = 0.22$
\[ 0.40  = 0.18 + 0.22 \]
\textbf{Remark:}  $M$ and $F$ are complement events.


\section{Bayes' Theorem}
Bayes' Theorem is a result that allows new information to be used to update the conditional probability of an event.
\bigskip

Recall the definition of conditional probability:
\[ P(A|B) = \frac{P(A \cap B)}{P(B)} \]


Using the multiplication rule, gives Bayes' Theorem in its simplest form:

\[ P(A|B) = \frac{P(B|A)\times P(A)}{P(B)} \]

%%%%%%%%%%%%%%%%%%%%%%%%%%%%%%%%%%%%%%%%%%%%%%%%%%%%%%%%%%%%%%%


Using the multiplication rule, gives Bayes' Theorem in its simplest form:

\[ P(A|B) = \frac{P(B|A)\times P(A)}{P(B)} \]


The general form of Bayes theorem is
\[ P(A|B) =
\frac{P(A \mbox{ and }B)}{P(B)} \]

Equivalently Bayes' Theorem can be expressed as
\begin{equation*}
P(B|A)=\frac{P\left(A|B\right) \times P(B) }{P\left( A\right) }.
\end{equation*}





\section{Conditional Probabilities}
Bayes Theorem


\[ P(A|B)  = \frac{P(A \mbox{and} B)}{P(B)} \]









\end{document}
